resolution is implies, not equals

dfy/cnf.dfy
@@ -20,6 +20,12 @@ ghost function cnf_equivalent(cnf: CNF, other: CNF) : (eq: bool)
         cnf_eval(cnf,vs) == cnf_eval(other, vs)
 }
 
+ghost function cnf_implies(cnf: CNF, other: CNF) : (eq: bool)
+{
+    forall vs : map<Variable, bool> :: true ==>
+        (cnf_eval(cnf,vs) ==> cnf_eval(other, vs))
+}
+
 predicate cnf_has_tautologies(cnf: CNF)
 {
     exists c :: c in cnf && clause_is_tautology(c)
@@ -32,35 +38,44 @@ function cnf_remove_tautologies(cnf: CNF) : (out: CNF)
     set c | c in cnf && !clause_is_tautology(c)
 }
 
-
 function clause_max_litvar(c: Clause) : (out: ClauseLit)
     requires |c| > 0
 {
-    if |c| == 1 then
-        Util.extract_only_from_set(c)
-    else
-        var lambda := (l: ClauseLit) => l.number();
-        SAT.NumbersBijection(c, lambda);
-        Util.extract_max_from_set(c, lambda)
+    var lambda := (l: ClauseLit) => l.number();
+    SAT.NumbersBijection(c, lambda);
+    Util.extract_max_from_set_by_score(c, lambda)
 }
 
-// function clause_gt(c1: Clause, c2: Clause) : (out: bool)
-//     requires c1 != c2
+function clause_lt(c1: Clause, c2: Clause) : (out: bool)
+    requires c1 != c2
+{
+    if |c1| < |c2| then
+        true
+    else if |c1| > |c2| then
+        false
+    else
+        var l1 := clause_max_litvar(c1);
+        var l2 := clause_max_litvar(c2);
+        if l1.number() < l2.number() then
+            true
+        else if l1.number() > l2.number() then
+            false
+        else
+            assert l1 == l2;
+            assert c1 - {l1} + {l1} == c1;
+            clause_lt(c1 - {l1}, c2 - {l2})
+}
+
+// lemma WellFormed(s: set<Clause>)
+//     ensures Util.well_ordered(s, (c1,c2) => clause_lt(c1,c2))
 // {
-//     if |c1| > |c2| then
-//         true
-//     else if |c1| < |c2| then
-//         false
-//     else
-//         assert |c1| == |c2|;
 
 // }
 
-// function max_clause(cs: set<Clause>) : (out: Clause)
-//     requires |cs| > 0
+// function max_clause(cnf: CNF) : (out: Clause)
+//     requires |cnf| > 0
 // {
-//     var c :| c in cs && forall cc :: cc in cs && cc != c ==>  c >= cc;
-//     c
+//     Util.extract_max_from_set_by_order(cnf, clause_lt)
 // }
 
 // function cnf_find_resolution_with_var(cnf: CNF, v: Variable) : (out: set<Clause>)
@@ -83,24 +98,124 @@ function clause_max_litvar(c: Clause) : (out: ClauseLit)
 //         {}
 // }
 
-// function cnf_has_resolution(cnf: CNF) : (out: bool)
-//     ensures out == (exists v :: v in cnf_vars(cnf) && cnf_has_resolution_with_var(cnf, v))
-// {
-//     exists v :: v in cnf_vars(cnf) && cnf_has_resolution_with_var(cnf, v)
-// }
+ghost function cnf_resolution_vars(cnf: CNF) : (out: set<Variable>)
+    ensures forall v :: v in out <==> v in cnf_vars(cnf) && cnf_has_resolution_with_var(cnf, v)
+{
+    set v | v in cnf_vars(cnf) && cnf_has_resolution_with_var(cnf, v)
+}
 
-// function cnf_has_resolution_with_var(cnf: CNF, v: Variable) : (out: bool)
-//     ensures out == (exists l1, l2, c1, c2 ::
-//         v in cnf_vars(cnf) &&
-//         c1 in cnf && c2 in cnf && c1 != c2 &&
-//         l1 in c1 && NotInverted(v) == l1 &&
-//         l2 in c2 && Inverted(v) == l2)
+function cnf_has_resolution(cnf: CNF) : (out: bool)
+    ensures out == (exists v :: v in cnf_vars(cnf) && cnf_has_resolution_with_var(cnf, v))
+{
+    exists v :: v in cnf_vars(cnf) && cnf_has_resolution_with_var(cnf, v)
+}
+
+function cnf_has_resolution_with_var(cnf: CNF, v: Variable) : (out: bool)
+{
+    exists c1, c2 ::
+        v in cnf_vars(cnf) &&
+        c1 in cnf && c2 in cnf && c1 != c2 &&
+        NotInverted(v) in c1 &&
+        Inverted(v) in c2
+}
+
+lemma BasicResolution(p: bool, q: bool, r: bool)
+    ensures ((p || q) && (!p || r)) ==> (q || r)
+{
+    
+}
+
+function merge_resolution_specific(v: Variable, vs: map<Variable, bool>, c1: Clause, c2: Clause) : (out: Clause)
+    requires v in vs
+    requires NotInverted(v) in c1 && Inverted(v) in c2
+    ensures (clause_eval(c1, vs) && clause_eval(c2, vs)) ==> clause_eval(out, vs)
+    ensures cnf_implies({c1, c2}, {out})
+{
+    var c1_others := c1 - {NotInverted(v)};
+    var c2_others := c2 - {Inverted(v)};
+    c1_others + c2_others
+}
+
+// function merge_resolution(v: Variable, c1: Clause, c2: Clause) : (out: Clause)
+//     requires NotInverted(v) in c1 && Inverted(v) in c2
+//     ensures cnf_equivalent({c1, c2}, {out})
 // {
-//     exists l1, l2, c1, c2 ::
-//         v in cnf_vars(cnf) &&
-//         c1 in cnf && c2 in cnf && c1 != c2 &&
-//         l1 in c1 && NotInverted(v) == l1 &&
-//         l2 in c2 && Inverted(v) == l2
+//     var orig := {c1, c2};
+
+//     var c1_others := c1 - {NotInverted(v)};
+//     assert forall vs :: v in vs ==> 
+//         clause_eval(c1, vs) == if vs[v] then
+//              true
+//         else
+//             clause_eval(c1_others, vs);
+//     assert forall vs :: v in vs ==> 
+//         clause_eval(c1, vs) == (vs[v] || clause_eval(c1_others, vs));
+
+//     var c2_others := c2 - {Inverted(v)};
+//     assert forall vs :: v in vs ==> 
+//         clause_eval(c2, vs) == if vs[v] then
+//              clause_eval(c2_others, vs)
+//         else
+//             true;
+//     assert forall vs :: v in vs ==> 
+//         clause_eval(c2, vs) == (!vs[v] || clause_eval(c2_others, vs));
+
+//     assert forall vs :: v in vs ==>
+//         BasicResolution(vs[v], clause_eval(c1_others, vs), clause_eval(c2_others, vs));
+//         assert (v[s] || clause_eval(c1_others, vs)) && (!v[s] || clause_eval(c2_others, vs)) == (clause_eval(c1_others, vs) || clause_eval(c2_others, vs));
+
+//     // assert forall vs :: v in vs ==> 
+//     //     if vs[v] then
+//     //         clause_eval(c1, vs) == 
+//     assert forall vs :: v in vs ==> 
+//         if vs[v] then
+//             cnf_eval(orig, vs) == cnf_eval({c2}, vs)
+//         else
+//             cnf_eval(orig, vs) == cnf_eval({c1}, vs);
+
+//     assert forall vs :: v in vs ==> 
+//         if vs[v] then
+//             cnf_eval(orig, vs) == cnf_eval({c2_others}, vs)
+//         else
+//             cnf_eval(orig, vs) == cnf_eval({c1_others}, vs);
+
+//     assert forall vs :: v in vs ==> 
+//         cnf_eval(orig, vs) ==
+//             if vs[v] then
+//                 cnf_eval({c2_others}, vs)
+//             else
+//                 cnf_eval({c1_others}, vs);
+
+//     assert forall vs :: v in vs ==> 
+//         cnf_eval(orig, vs) ==
+//             if vs[v] then
+//                 clause_eval(c2_others, vs)
+//             else
+//                 clause_eval(c1_others, vs);
+    
+//     assert forall vs :: v in vs ==> 
+//         cnf_eval(orig, vs) ==
+//             (clause_eval(c2_others, vs) || clause_eval(c1_others, vs));
+
+//     // assert forall vs :: v in vs ==> 
+//     //     cnf_eval(orig, vs) == (clause_eval(c1, vs) && clause_eval(c2, vs));
+        
+//     // assert forall vs :: v in vs ==> 
+//     //     (   cnf_eval(orig, vs) == cnf_eval({c1_others}, vs) 
+//     //      || cnf_eval(orig, vs) == cnf_eval({c2_others}, vs));
+
+//     // assert forall vs :: v in vs ==> 
+//     //     cnf_eval(orig, vs) == cnf_eval({c1_others + c2_others}, vs);
+
+//     assert forall vs :: v in vs ==>
+//         (clause_eval(c1_others, vs) || clause_eval(c2_others, vs)) == clause_eval(c1_others + c2_others, vs);
+
+
+//     assert forall vs :: v in vs ==> 
+//         cnf_eval(orig, vs) == cnf_eval({c1_others + c2_others}, vs);
+        
+//     var merged := c1_others + c2_others;
+//     merged
 // }
 
 // ghost function cnf_some_resolution_var(cnf: CNF) : (v: Variable)
@@ -121,6 +236,48 @@ function clause_max_litvar(c: Clause) : (out: ClauseLit)
 //     set c | c in cnf && (exists l :: l in ls && l in c)
 // }
 
+lemma SetSetWithSomethingInItIsNotEmpty<T>(s: set<T>, f: T -> bool, ss: set<T>)
+    requires exists x :: x in s && f(x)
+    requires ss == set x | x in s && f(x)
+    ensures |ss| > 0
+{
+    var x :| x in s && f(x);
+    assert x in s;
+    assert f(x);
+    assert x in ss;
+    assert |ss| > 0;
+}
+
+function cnf_resolution(cnf: CNF) : (out: CNF)
+    requires !cnf_has_tautologies(cnf)
+    ensures !cnf_has_resolution(out)
+    ensures cnf_equivalent(cnf, out)
+{
+    // no tautologies
+    assert forall v, l1, l2, c ::
+        v in cnf_vars(cnf) &&
+        c in cnf &&
+        l1 in c && l2 in c ==>
+            l1.invert() != l2;
+
+    var resolutions: set<(Variable, Clause, Clause)> := set v,c1,c2 
+        | v in cnf_vars(cnf) && c1 in cnf && c2 in cnf && c1 != c2 &&
+            NotInverted(v) in c1 && Inverted(v) in c2
+        :: (v, c1, c2);
+    assert forall r :: r in resolutions ==> (
+        assert r.0 in cnf_vars(cnf);
+        assert exists c1, c2 :: 
+            r.0 in cnf_vars(cnf) &&
+            c1 in cnf && c2 in cnf && c1 != c2
+            && NotInverted(r.0) in c1 && Inverted(r.0) in c2;
+
+        cnf_has_resolution_with_var(cnf, r.0)
+        );
+    
+    assume false;
+    cnf
+}
+
 // function cnf_resolution(cnf: CNF) : (out: CNF)
 //     requires !cnf_has_tautologies(cnf)
 //     requires cnf_has_resolution(cnf)
@@ -133,8 +290,14 @@ function clause_max_litvar(c: Clause) : (out: ClauseLit)
 //         l2 in c2 && Inverted(v) == l2;
 //     assert exists c :: c in cnf && NotInverted(v) in c;
 
-//     var where_not_inverted: set<Clause> := set c | c in cnf && NotInverted(v) in c;
+//     var f :=  (c: Clause) => NotInverted(v) in c;
+//     var where_not_inverted: set<Clause> := set c | c in cnf && f(c);
+//     assert exists c :: c in cnf && f(c);
+//     SetSetWithSomethingInItIsNotEmpty(cnf, f, where_not_inverted);
+//     assume false;
 //     assert |where_not_inverted| > 0;
+
+
 //     // var where_inverted: set<Clause> := set c | c in cnf && Inverted(v) in c;
 //     // assert |where_inverted| > 0;
 
